test/test.ml
@@ -1,8 +1,8 @@
 let () =
-  let t = Elias_fano.encode ~universe:100 [3; 7; 42] in
+  let t = Elias_fano.encode ~universe:100 [|3; 7; 42|] in
 
   (* round-trip *)
-  assert (Elias_fano.decode t = [3; 7; 42]);
+  assert (Elias_fano.decode t = [|3; 7; 42|]);
 
   (* access *)
   assert (Elias_fano.access t 0 = 3);
@@ -16,16 +16,16 @@ let () =
   assert (Elias_fano.next_geq t 0 = Some 3);
 
   (* larger example *)
-  let t2 = Elias_fano.encode ~universe:1000 [0; 1; 2; 3; 4; 5] in
-  assert (Elias_fano.decode t2 = [0; 1; 2; 3; 4; 5]);
+  let t2 = Elias_fano.encode ~universe:1000 [|0; 1; 2; 3; 4; 5|] in
+  assert (Elias_fano.decode t2 = [|0; 1; 2; 3; 4; 5|]);
 
-  let t3 = Elias_fano.encode ~universe:256 [10; 20; 30; 100; 200; 255] in
-  assert (Elias_fano.decode t3 = [10; 20; 30; 100; 200; 255]);
+  let t3 = Elias_fano.encode ~universe:256 [|10; 20; 30; 100; 200; 255|] in
+  assert (Elias_fano.decode t3 = [|10; 20; 30; 100; 200; 255|]);
 
   (* edge cases *)
-  assert (Elias_fano.decode (Elias_fano.encode ~universe:1 []) = []);
-  assert (Elias_fano.decode (Elias_fano.encode ~universe:10 [0]) = [0]);
-  assert (Elias_fano.decode (Elias_fano.encode ~universe:100 [0; 0; 0]) = [0; 0; 0]);
+  assert (Elias_fano.decode (Elias_fano.encode ~universe:1 [||]) = [||]);
+  assert (Elias_fano.decode (Elias_fano.encode ~universe:10 [|0|]) = [|0|]);
+  assert (Elias_fano.decode (Elias_fano.encode ~universe:100 [|0; 0; 0|]) = [|0; 0; 0|]);
 
   (* bit_size *)
   assert (Elias_fano.bit_size t = 21);
